compiler/backend/passes/pure_letrec_cexpScript.sml
@@ -14,10 +14,10 @@ val _ = new_theory "pure_letrec_cexp";
 Definition letrec_recurse_cexp_def:
   letrec_recurse_cexp f (Letrec c xs y) =
     f c (MAP (λ(n,x). n, letrec_recurse_cexp f x) xs) (letrec_recurse_cexp f y) ∧
-  letrec_recurse_cexp f (Lam c ns x) = Lam c ns (letrec_recurse_cexp f x) ∧
+  letrec_recurse_cexp f (Lam c ns x) = SmartLam c ns (letrec_recurse_cexp f x) ∧
   letrec_recurse_cexp f (Prim c p xs) = Prim c p (MAP (letrec_recurse_cexp f) xs) ∧
   letrec_recurse_cexp f (App c x ys) =
-    App c (letrec_recurse_cexp f x) (MAP (letrec_recurse_cexp f) ys) ∧
+    SmartApp c (letrec_recurse_cexp f x) (MAP (letrec_recurse_cexp f) ys) ∧
   letrec_recurse_cexp f (Var c v) = Var c v ∧
   letrec_recurse_cexp f (Let c n x y) =
     Let c n (letrec_recurse_cexp f x) (letrec_recurse_cexp f y) ∧
